# wasfnabsfsa  

$(P\iff Q) = ((P\implies Q) \land (Q\implies P))$  

$\lnot(P\iff Q) = \lnot((P\implies Q) \land (Q\implies P))$  
$=\lnot(P\implies Q) \lor \lnot(Q\implies P)$  
$=(P\land \lnot Q) \lor (Q\land \lnot P)$  
$=P\oplus Q=(P\iff \lnot Q)$  

$(x \geq 3) \iff [(x>3) \lor (x=3)]$.  
Negated: $(x \geq 3) \iff \lnot[(x>3) \lor (x=3)]$.  
$\iff (x\leq 3)\land(x\neq 3)$
$\iff x<3$.  
Final negated: $(x\geq3) \iff (x<3)$.  

If $A\subseteq B$ and $B\subseteq C$, then $A\subseteq C$

Proof.  
There are two cases:  
$A=\emptyset$  
$\exists x\in A$  

Case 1: $A=\empty$  

If $A=\empty$, $A$ must be the subset of set C, as $\empty$ is the subset of *all sets*, including itself. THerefore, $A\subseteq C$.  

Case 2: $A\neq\empty$  

The definition of a subset states that $A\subseteq B$ *if and only if* $n\in A \implies n\in B$.  
That is, the following are true:  
$A\subseteq B \implies (x\in A \implies x\in B)$
$(x\in A \implies x\in B) \implies A\subseteq B$

Let $x\in A$, $A\subseteq B$ and $B\subseteq C$.  
Since $A\subseteq B$, by definition of a subset, $x\in A \implies x\in B$.  
Following the same reasoning, since $B\subseteq C$, $x\in B \implies x\in C$.  
If $x\in A \implies x\in B$, and $x\in B \implies x\in C$, then $x\in A \implies x\in C$.  
We have shown that if $A\subseteq B$ and $B \subseteq C$, then $x\in A \implies x\in C$, which by definition means $A\subseteq C$.  
QED.  