# sdgdsg

A function $f$ is injective if $a\neq b \implies f(a)\neq f(b)$.  
$f(a)=f(b)\implies a=b$.  

Given a bijection $f: A\to B$  
and $a\in A$, the function  
$g: A-\{a\} \to B-\{f(a)\}$ 
defined by  
$g(a')=f(a')$ if $a'\neq a$
is well defined and bijective.  


.. blah blah proof that it is well defined. i took a picture of it

**First, prove $g$ is injective.**  
Let $a', a''\in A-\{a\}$ such that $g(a')=g(a'')$.  
We want to prove $a'=a''$.  
Since $g(a')=f(a')$ and $g(a'')=f(a'')$, we know $f(a')=f(a'')$.  
Since $f$ is injective, $a'=a''$.  
$\therefore g$ is injective.  

**Next, prove $g$ is surjective.**  
$g$ is surjective if for all $b'\in B-\{f(a)\}$, there exists a $a'\in A-\{a\}$ such that $g(a')=b'$.  

Let $b'\in B-\{f(a)\}$.  
Since $f$ is surjective, $\exists a'\in A$ such that $b'=f(a')$.  
If $a'=a$, then $g(a')=f(a')=f(a)$ since $f$ is bijective, which is not in $B-\{f(a)\}$. This can't occur bc $f(a')=g(a')=b'\in B-\{f(a)\}$. Therefore, $a'\neq a$, and $a'\in A-\{a\}$.  
